aneris/examples/transactional_consistency/snapshot_isolation/specs/specs.v
@@ -24,63 +24,61 @@ Section Specification.
   Context `{!anerisG Mdl Σ, !User_params,
             !KVS_transaction_api, !SI_resources Mdl Σ}.
 
-  Definition write_spec : Prop :=
-    ∀ (c : val) (sa : socket_address)
-      (vo : option val)
-      (k : Key) (v : SerializableVal) (b : bool) ,
-      ⌜k ∈ KVS_keys⌝ -∗
-      IsConnected c sa -∗
+  Definition write_spec : iProp Σ :=
+    □ ∀ (c : val) (sa : socket_address)
+    (vo : option val)
+    (k : Key) (v : SerializableVal) (b : bool) ,
+    ⌜k ∈ KVS_keys⌝ -∗
+    IsConnected c sa -∗
     {{{ k ↦{c} vo ∗ KeyUpdStatus c k b}}}
       TC_write c #k v @[ip_of_address sa] 
     {{{ RET #(); k ↦{c} Some v.(SV_val) ∗ KeyUpdStatus c k true }}}.
 
-  Definition read_spec : Prop :=
-    ∀ (c : val) (sa : socket_address)
-      (k : Key) (vo : option val),
+  Definition read_spec : iProp Σ :=
+    □ ∀ (c : val) (sa : socket_address)
+    (k : Key) (vo : option val),
     ⌜k ∈ KVS_keys⌝ -∗
     IsConnected c sa -∗
     {{{ k ↦{c} vo }}}
       TC_read c #k @[ip_of_address sa] 
     {{{ RET $vo; k ↦{c} vo }}}.
 
-   Definition start_spec : Prop :=
-    ∀ (c : val) (sa : socket_address)
-       (E : coPset),
-      ⌜↑KVS_InvName ⊆ E⌝ -∗
-      IsConnected c sa -∗
+   Definition start_spec : iProp Σ :=
+    □ ∀ (c : val) (sa : socket_address)
+    (E : coPset),
+    ⌜↑KVS_InvName ⊆ E⌝ -∗
+    IsConnected c sa -∗
     <<< ∀∀ (m : gmap Key Hist),
-       ConnectionState c sa CanStart ∗
-       [∗ map] k ↦ h ∈ m, k ↦ₖ h >>>
+      ConnectionState c sa CanStart ∗
+      [∗ map] k ↦ h ∈ m, k ↦ₖ h >>>
       TC_start c @[ip_of_address sa] E
     <<<▷ RET #();
-       ConnectionState c sa (Active m) ∗
-       ([∗ map] k ↦ h ∈ m, k ↦ₖ h) ∗
-       ([∗ map] k ↦ h ∈ m, k ↦{c} (last h) ∗ KeyUpdStatus c k false) ∗
-       ([∗ map] k ↦ h ∈ m, Seen k h)>>>.
+      ConnectionState c sa (Active m) ∗
+      ([∗ map] k ↦ h ∈ m, k ↦ₖ h) ∗
+      ([∗ map] k ↦ h ∈ m, k ↦{c} (last h) ∗ KeyUpdStatus c k false) ∗
+      ([∗ map] k ↦ h ∈ m, Seen k h) >>>.
 
-  Definition commit_spec : Prop :=
-   ∀ (c : val) (sa : socket_address)
-     (E : coPset),
-     ⌜↑KVS_InvName ⊆ E⌝ -∗
-     IsConnected c sa -∗
-    <<< ∀∀ (m ms: gmap Key Hist)
-           (mc : gmap Key (option val * bool)),
-        ConnectionState c sa (Active ms) ∗
-        ⌜dom m = dom ms⌝ ∗ ⌜dom ms = dom mc⌝ ∗
-        ([∗ map] k ↦ h ∈ m, k ↦ₖ h) ∗
-        ([∗ map] k ↦ p ∈ mc, k ↦{c} p.1  ∗ KeyUpdStatus c k p.2) >>>
+  Definition commit_spec : iProp Σ :=
+    □ ∀ (c : val) (sa : socket_address)
+    (E : coPset),
+    ⌜↑KVS_InvName ⊆ E⌝ -∗
+    IsConnected c sa -∗
+    <<< ∀∀ (m ms: gmap Key Hist) (mc : gmap Key (option val * bool)),
+      ConnectionState c sa (Active ms) ∗
+      ⌜dom m = dom ms⌝ ∗ ⌜dom ms = dom mc⌝ ∗
+      ([∗ map] k ↦ h ∈ m, k ↦ₖ h) ∗
+      ([∗ map] k ↦ p ∈ mc, k ↦{c} p.1  ∗ KeyUpdStatus c k p.2) >>>
       TC_commit c @[ip_of_address sa] E
     <<<▷∃∃ b, RET #b;
-        ConnectionState c sa CanStart ∗
-        (** Transaction has been commited. *)
-        ((⌜b = true⌝ ∗ ⌜can_commit m ms mc⌝ ∗
-          ([∗ map] k↦ h;p ∈ m; mc,
-            k ↦ₖ commit_event p h ∗ Seen k (commit_event p h))) ∨
-        (** Transaction has been aborted. *)
-         (⌜b = false⌝ ∗ ⌜¬ can_commit m ms mc⌝ ∗
-           [∗ map] k ↦ h ∈ m, k ↦ₖ h ∗ Seen k h)) >>>.
+      ConnectionState c sa CanStart ∗
+      (** Transaction has been commited. *)
+      ((⌜b = true⌝ ∗ ⌜can_commit m ms mc⌝ ∗
+        ([∗ map] k↦ h;p ∈ m; mc, k ↦ₖ commit_event p h ∗ Seen k (commit_event p h))) ∨
+      (** Transaction has been aborted. *)
+      (⌜b = false⌝ ∗ ⌜¬ can_commit m ms mc⌝ ∗
+        [∗ map] k ↦ h ∈ m, k ↦ₖ h ∗ Seen k h)) >>>.
 
-  Definition init_client_proxy_spec : Prop :=
+  Definition init_client_proxy_spec : iProp Σ :=
     ∀ (sa : socket_address),
     {{{ unallocated {[sa]} ∗
         KVS_address ⤇ KVS_si ∗
@@ -92,16 +90,16 @@ Section Specification.
     {{{ cstate, RET cstate; ConnectionState cstate sa CanStart ∗
                             IsConnected cstate sa }}}.
 
-  Definition init_kvs_spec : Prop :=
-  {{{ KVS_address ⤇ KVS_si ∗
-        KVS_address ⤳ (∅,∅) ∗
-        free_ports (ip_of_address KVS_address)
-                   {[port_of_address KVS_address]} ∗
-      KVS_Init }}}
-      TC_init_server (s_serializer KVS_serialization)
-        #KVS_address
-        @[(ip_of_address KVS_address)]
-    {{{ RET #(); True }}}.
+  Definition init_kvs_spec : iProp Σ :=
+    {{{ KVS_address ⤇ KVS_si ∗
+          KVS_address ⤳ (∅,∅) ∗
+          free_ports (ip_of_address KVS_address)
+                    {[port_of_address KVS_address]} ∗
+        KVS_Init }}}
+        TC_init_server (s_serializer KVS_serialization)
+          #KVS_address
+          @[(ip_of_address KVS_address)]
+      {{{ RET #(); True }}}.
 
 End Specification.
 
@@ -110,12 +108,12 @@ Section SI_Module.
             !KVSG Σ, !KVS_transaction_api}.
 
   Class SI_client_toolbox `{!SI_resources Mdl Σ} := {
-    SI_init_kvs_spec : init_kvs_spec ;
-    SI_init_client_proxy_spec : init_client_proxy_spec;
-    SI_read_spec : read_spec ;
-    SI_write_spec : write_spec;
-    SI_start_spec : start_spec;
-    SI_commit_spec : commit_spec;
+    SI_init_kvs_spec : ⊢ init_kvs_spec ;
+    SI_init_client_proxy_spec : ⊢ init_client_proxy_spec;
+    SI_read_spec : ⊢ read_spec ;
+    SI_write_spec : ⊢ write_spec;
+    SI_start_spec : ⊢ start_spec;
+    SI_commit_spec : ⊢ commit_spec;
   }.
  
    Class SI_init := {
@@ -127,13 +125,12 @@ Section SI_Module.
         KVS_Init ∗
         GlobalInv ∗
         ([∗ set] sa ∈ clients, KVS_ClientCanConnect sa) ∗
-        ⌜init_kvs_spec⌝ ∗
-        ⌜init_client_proxy_spec⌝ ∗
-        ⌜read_spec⌝ ∗
-        ⌜write_spec⌝ ∗
-        ⌜start_spec⌝ ∗
-        ⌜commit_spec⌝
+        init_kvs_spec ∗
+        init_client_proxy_spec ∗
+        read_spec ∗
+        write_spec ∗
+        start_spec ∗
+        commit_spec
      }.
    
 End SI_Module.
- 
