aneris/examples/transactional_consistency/snapshot_isolation/examples/deprecated/causality_example/causality_example_proof.v
@@ -1,4 +1,4 @@
-From aneris.aneris_lang Require Import network resources proofmode.
+(* From aneris.aneris_lang Require Import network resources proofmode.
 From aneris.aneris_lang.lib.serialization
      Require Import serialization_proof.
 From aneris.aneris_lang.lib Require Import inject.
@@ -515,4 +515,4 @@ Proof.
   do 3 (rewrite big_sepS_union; [|set_solver];
   rewrite !big_sepS_singleton;
   iDestruct "Hips" as "[Hips ?]"; iFrame).
-Qed. 
+Qed.  *)
