aneris/examples/transactional_consistency/snapshot_isolation/examples/deprecated/classical_example_run/classical_example_run_derived_simple_proof.v
@@ -1,4 +1,4 @@
-From aneris.aneris_lang Require Import network resources proofmode.
+(* From aneris.aneris_lang Require Import network resources proofmode.
 From aneris.aneris_lang.lib Require Import
      list_proof inject lock_proof.
 From aneris.aneris_lang.lib.serialization
@@ -10,7 +10,7 @@ From aneris.aneris_lang.program_logic Require Import
      aneris_weakestpre aneris_adequacy aneris_lifting.
 From iris.base_logic.lib Require Import invariants.
 From aneris.examples.transactional_consistency.snapshot_isolation.specs Require Import
-  time events aux_defs resources specs derived_specs.
+  derived_specs time events aux_defs resources specs.
 From aneris.examples.transactional_consistency.snapshot_isolation.examples.classical_example_run
       Require Import classical_example_run_code.
 Import ser_inj.
@@ -77,46 +77,39 @@ Context `{!anerisG Mdl Σ, !SI_resources Mdl Σ, !SI_client_toolbox}.
     { iPureIntro. apply SI_init_client_proxy_spec. }
     iIntros (rpc) "(Hcstate & #HiC)".
     wp_pures.
-    wp_apply (run_spec_derived_generic rpc _ client_1_addr (⊤ ∖ ↑client_inv_name)
+    wp_apply (run_spec_derived_simple rpc _ KVS_keys client_1_addr (⊤ ∖ ↑client_inv_name)
       (λ msnap, ⌜∃ vo, msnap = {["x" := vo; "y" := vo]}⌝)%I 
-      (λ _ msnap mc, ⌜mc = {["x" := (Some #1, true); "y" := (Some #1, true)]}⌝)%I
-      with "[][][][][$Hcstate][HΦ]"); try solve_ndisj.
+      (λ mc, ⌜mc = {["x" := (Some #1, true); "y" := (Some #1, true)]}⌝)%I
+      with "[][][][][][][$Hcstate][HΦ]"); try solve_ndisj.
     - iPureIntro. apply SI_start_spec. 
-    - iPureIntro. apply SI_commit_spec.
-    - iSplit.
-      + iInv (client_inv_name) as ">[%h[Hx Hy]]" "HClose".
-        iModIntro. iExists {["x" := h; "y" := h]}.
-        iSplit. { iPureIntro. by exists h. }
-        rewrite !big_sepM_insert; try set_solver.
-        rewrite big_sepM_empty. iFrame.
-        iNext. iIntros "(Hx & Hy & _)".
-        iMod ("HClose" with "[Hx Hy]") as "_"; last done.
-        iNext. iExists h. iFrame.
-      + iIntros (msnap Φ') "!# (H_cache & [%h ->]) HΦ'".
-        rewrite /transaction1. wp_pures.
-        rewrite !big_sepM_insert; try set_solver.
-        iDestruct "H_cache" as "(H_cx & H_cy & _)".
-        wp_apply (SI_write_spec _ _ _ _ (SerVal #1) with "[][$][H_cx]").
-        set_solver. iFrame "#∗". iIntros "Hcx". wp_pures.
-        wp_apply (SI_write_spec _ _ _ _ (SerVal #1) with "[][$][H_cy]").
-        set_solver. iFrame "#∗". iIntros "Hcy".
-        iApply ("HΦ'" $! {["x" := (Some #1, true); "y" := (Some #1, true)]}).
-        iSplit. { iPureIntro. set_solver. }
-        iSplitL.
-        { rewrite !big_sepM_insert; try set_solver. rewrite big_sepM_empty. iFrame. }
-        iInv (client_inv_name) as ">[%h'[Hx Hy]]" "HClose".
-        iModIntro. iExists {["x" := h'; "y" := h']}.
-        rewrite !big_sepM_insert; try set_solver.
-        rewrite big_sepM_empty. iFrame.
-        iSplit. { iPureIntro. set_solver. }
-        iSplit. { iPureIntro. set_solver. }
-        iIntros ">[ Hkeys | (Hx & Hy & _)]".
-        * iMod ("HClose" with "[Hkeys]") as "_"; last done.
-          iNext. iExists (Some (#1)).
-          rewrite !big_sepM2_insert; try set_solver.
-          iDestruct "Hkeys" as "(Hx & Hy & _)". iFrame.
-        * iMod ("HClose" with "[Hx Hy]") as "_"; last done.
-          iNext. iExists h'. iFrame.
+    - iPureIntro. apply SI_commit_spec. 
+    - iModIntro.
+      iInv (client_inv_name) as ">[%vo[Hx Hy]]" "HClose".
+      iModIntro. iExists {["x" := vo; "y" := vo]}.
+      iSplit. { iPureIntro. set_solver. }
+      iSplit. { iPureIntro. by exists vo. }
+      rewrite !big_sepM_insert; try set_solver.
+      rewrite big_sepM_empty. iFrame.
+      iNext. iIntros "[ [%m_cache (-> & Hkeys)] | (Hx & Hy & _)]".
+      + iMod ("HClose" with "[Hkeys]") as "_"; last done.
+        iNext. iExists (Some #1).
+        rewrite !big_sepM2_insert; try set_solver.
+        iDestruct "Hkeys" as "(Hx & Hy & _)". iFrame.
+      + iMod ("HClose" with "[Hx Hy]") as "_"; last done.
+        iNext. iExists vo. iFrame.
+    - iIntros (msnap Φ') "!# (H_cache & [%h ->]) HΦ'".
+      rewrite /transaction1. wp_pures.
+      rewrite !big_sepM_insert; try set_solver.
+      iDestruct "H_cache" as "(H_cx & H_cy & _)".
+      wp_apply (SI_write_spec  _ _ _ _ (SerVal #1) with "[][$][H_cx]").
+      set_solver. iFrame "#∗". iIntros "Hcx". wp_pures.
+      wp_apply (SI_write_spec  _ _ _ _ (SerVal #1) with "[][$][H_cy]").
+      set_solver. iFrame "#∗". iIntros "Hcy".
+      iApply ("HΦ'" $! {["x" := (Some #1, true); "y" := (Some #1, true)]}).
+      iSplit. { iPureIntro. set_solver. }
+      iSplit; last done.
+      rewrite !big_sepM_insert; try set_solver.
+      rewrite big_sepM_empty. iFrame.
     - iNext. iIntros. by iApply "HΦ".
   Qed.
 
@@ -139,46 +132,39 @@ Context `{!anerisG Mdl Σ, !SI_resources Mdl Σ, !SI_client_toolbox}.
     { iPureIntro. apply SI_init_client_proxy_spec. }
     iIntros (rpc) "(Hcstate & #HiC)".
     wp_pures.
-    wp_apply (run_spec_derived_generic rpc _ client_2_addr (⊤ ∖ ↑client_inv_name)
+    wp_apply (run_spec_derived_simple rpc _ KVS_keys client_2_addr (⊤ ∖ ↑client_inv_name)
       (λ msnap, ⌜∃ vo, msnap = {["x" := vo; "y" := vo]}⌝)%I 
-      (λ _ msnap mc, ⌜mc = {["x" := (Some #2, true); "y" := (Some #2, true)]}⌝)%I
-      with "[][][][][$Hcstate][HΦ]"); try solve_ndisj.
+      (λ mc, ⌜mc = {["x" := (Some #2, true); "y" := (Some #2, true)]}⌝)%I
+      with "[][][][][][][$Hcstate][HΦ]"); try solve_ndisj.
     - iPureIntro. apply SI_start_spec. 
-    - iPureIntro. apply SI_commit_spec.
-    - iSplit.
-      + iInv (client_inv_name) as ">[%h[Hx Hy]]" "HClose".
-        iModIntro. iExists {["x" := h; "y" := h]}.
-        iSplit. { iPureIntro. by exists h. }
-        rewrite !big_sepM_insert; try set_solver.
-        rewrite big_sepM_empty. iFrame.
-        iNext. iIntros "(Hx & Hy & _)".
-        iMod ("HClose" with "[Hx Hy]") as "_"; last done.
-        iNext. iExists h. iFrame.
-      + iIntros (msnap Φ') "!# (H_cache & [%h ->]) HΦ'".
-        rewrite /transaction2. wp_pures.
-        rewrite !big_sepM_insert; try set_solver.
-        iDestruct "H_cache" as "(H_cx & H_cy & _)".
-        wp_apply (SI_write_spec _ _ _ _ (SerVal #2) with "[][$][H_cx]").
-        set_solver. iFrame "#∗". iIntros "Hcx". wp_pures.
-        wp_apply (SI_write_spec _ _ _ _ (SerVal #2) with "[][$][H_cy]").
-        set_solver. iFrame "#∗". iIntros "Hcy".
-        iApply ("HΦ'" $! {["x" := (Some #2, true); "y" := (Some #2, true)]}).
-        iSplit. { iPureIntro. set_solver. }
-        iSplitL.
-        { rewrite !big_sepM_insert; try set_solver. rewrite big_sepM_empty. iFrame. }
-        iInv (client_inv_name) as ">[%h'[Hx Hy]]" "HClose".
-        iModIntro. iExists {["x" := h'; "y" := h']}.
-        rewrite !big_sepM_insert; try set_solver.
-        rewrite big_sepM_empty. iFrame.
-        iSplit. { iPureIntro. set_solver. }
-        iSplit. { iPureIntro. set_solver. }
-        iIntros ">[ Hkeys | (Hx & Hy & _)]".
-        * iMod ("HClose" with "[Hkeys]") as "_"; last done.
-          iNext. iExists (Some (#2)).
-          rewrite !big_sepM2_insert; try set_solver.
-          iDestruct "Hkeys" as "(Hx & Hy & _)". iFrame.
-        * iMod ("HClose" with "[Hx Hy]") as "_"; last done.
-          iNext. iExists h'. iFrame.
+    - iPureIntro. apply SI_commit_spec. 
+    - iModIntro.
+      iInv (client_inv_name) as ">[%vo[Hx Hy]]" "HClose".
+      iModIntro. iExists {["x" := vo; "y" := vo]}.
+      iSplit. { iPureIntro. set_solver. }
+      iSplit. { iPureIntro. by exists vo. }
+      rewrite !big_sepM_insert; try set_solver.
+      rewrite big_sepM_empty. iFrame.
+      iNext. iIntros "[ [%m_cache (-> & Hkeys)] | (Hx & Hy & _)]".
+      + iMod ("HClose" with "[Hkeys]") as "_"; last done.
+        iNext. iExists (Some #2).
+        rewrite !big_sepM2_insert; try set_solver.
+        iDestruct "Hkeys" as "(Hx & Hy & _)". iFrame.
+      + iMod ("HClose" with "[Hx Hy]") as "_"; last done.
+        iNext. iExists vo. iFrame.
+    - iIntros (msnap Φ') "!# (H_cache & [%h ->]) HΦ'".
+      rewrite /transaction2. wp_pures.
+      rewrite !big_sepM_insert; try set_solver.
+      iDestruct "H_cache" as "(H_cx & H_cy & _)".
+      wp_apply (SI_write_spec  _ _ _ _ (SerVal #2) with "[][$][H_cx]").
+      set_solver. iFrame "#∗". iIntros "Hcx". wp_pures.
+      wp_apply (SI_write_spec  _ _ _ _ (SerVal #2) with "[][$][H_cy]").
+      set_solver. iFrame "#∗". iIntros "Hcy".
+      iApply ("HΦ'" $! {["x" := (Some #2, true); "y" := (Some #2, true)]}).
+      iSplit. { iPureIntro. set_solver. }
+      iSplit; last done.
+      rewrite !big_sepM_insert; try set_solver.
+      rewrite big_sepM_empty. iFrame.
     - iNext. iIntros. by iApply "HΦ".
   Qed.
 
@@ -201,63 +187,47 @@ Context `{!anerisG Mdl Σ, !SI_resources Mdl Σ, !SI_client_toolbox}.
     { iPureIntro. apply SI_init_client_proxy_spec. }
     iIntros (rpc) "(Hcstate & #HiC)".
     wp_pures.
-    wp_apply (run_spec_derived_generic rpc _ client_3_addr (⊤ ∖ ↑client_inv_name)
+    wp_apply (run_spec_derived_simple rpc _ KVS_keys client_3_addr (⊤ ∖ ↑client_inv_name)
       (λ msnap, ⌜∃ vo, msnap = {["x" := vo; "y" := vo]}⌝)%I 
-      (λ _ msnap mc, ⌜∃ vo1 vo2, mc = {["x" := (vo1, false); "y" := (vo2, false)]}⌝)%I
-      with "[][][][][$Hcstate][HΦ]"); try solve_ndisj.
+      (λ mc, ⌜∃ vo1 vo2, mc = {["x" := (vo1, false); "y" := (vo2, false)]}⌝)%I
+      with "[][][][][][][$Hcstate][HΦ]"); try solve_ndisj.
     - iPureIntro. apply SI_start_spec. 
-    - iPureIntro. apply SI_commit_spec.
-    - iSplit.
-      + iInv (client_inv_name) as ">[%vo[Hx Hy]]" "HClose".
-        iModIntro. iExists {["x" := vo; "y" := vo]}.
-        iSplit. { iPureIntro. by exists vo. }
+    - iPureIntro. apply SI_commit_spec. 
+    - iModIntro.
+      iInv (client_inv_name) as ">[%vo[Hx Hy]]" "HClose".
+      iModIntro. iExists {["x" := vo; "y" := vo]}.
+      iSplit. { iPureIntro. set_solver. }
+      iSplit. { iPureIntro. by exists vo. }
+      rewrite !big_sepM_insert; try set_solver.
+      rewrite big_sepM_empty. iFrame.
+      iNext. iIntros "[ [%m_cache ([%vo1 [%vo2 ->]] & Hkeys)] | (Hx & Hy & _)]".
+      + iMod ("HClose" with "[Hkeys]") as "_"; last done.
+        iNext. iExists vo.
+        rewrite !big_sepM2_insert; try set_solver.
+        iDestruct "Hkeys" as "(Hx & Hy & _)". iFrame.
+        destruct vo1, vo2; iFrame.
+      + iMod ("HClose" with "[Hx Hy]") as "_"; last done.
+        iNext. iExists vo. iFrame.
+    - iIntros (msnap Φ') "!# (H_cache & [%vo ->]) HΦ'".
+      rewrite /transaction3. wp_pures.
+      rewrite !big_sepM_insert; try set_solver.
+      iDestruct "H_cache" as "((H_cx & H_cx_s) & (H_cy & H_cy_s) & _)".
+      wp_apply (SI_read_spec _ _ _ _ with "[][$][H_cx]"); try set_solver.
+      iFrame "#∗". iIntros "H_cx". wp_pures.
+      wp_apply (SI_read_spec _ _ _ _ with "[][$][H_cy]"); try set_solver.
+      iFrame "#∗". iIntros "H_cy". wp_pures.
+      destruct vo; do 2 wp_lam; wp_pures. 
+      + case_bool_decide as Heq; try set_solver. wp_pures.
+        iApply ("HΦ'" $! {["x" := (Some v, false); "y" := (Some v, false)]}).
+        iSplit. { iPureIntro. set_solver. }
+        iSplit; last set_solver.
         rewrite !big_sepM_insert; try set_solver.
         rewrite big_sepM_empty. iFrame.
-        iNext. iIntros "(Hx & Hy & _)".
-        iMod ("HClose" with "[Hx Hy]") as "_"; last done.
-        iNext. iExists vo. iFrame.
-      + iIntros (msnap Φ') "!# (H_cache & [%vo ->]) HΦ'".
-        rewrite /transaction3. wp_pures.
+      + iApply ("HΦ'" $! {["x" := (None, false); "y" := (None, false)]}).
+        iSplit. { iPureIntro. set_solver. }
+        iSplit; last set_solver.
         rewrite !big_sepM_insert; try set_solver.
-        iDestruct "H_cache" as "((H_cx & H_cx_s) & (H_cy & H_cy_s) & _)".
-        wp_apply (SI_read_spec _ _ _ _ with "[][$][H_cx]"); try set_solver.
-        iFrame "#∗". iIntros "H_cx". wp_pures.
-        wp_apply (SI_read_spec _ _ _ _ with "[][$][H_cy]"); try set_solver.
-        iFrame "#∗". iIntros "H_cy". wp_pures.
-        destruct vo; do 2 wp_lam; wp_pures. 
-        * case_bool_decide as Heq; try set_solver. wp_pures.
-          iApply ("HΦ'" $! {["x" := (Some v, false); "y" := (Some v, false)]}).
-          iSplit. { iPureIntro. set_solver. }
-          iSplitL. {rewrite !big_sepM_insert; try set_solver. rewrite big_sepM_empty. iFrame. }
-          iInv (client_inv_name) as ">[%vo'[Hx Hy]]" "HClose".
-          iModIntro. iExists {["x" := vo'; "y" := vo']}.
-          rewrite !big_sepM_insert; try set_solver.
-          rewrite big_sepM_empty. iFrame.
-          iSplit. { iPureIntro. set_solver. }
-          iSplit. { iPureIntro. set_solver. }
-          iIntros ">[ Hkeys | (Hx & Hy & _)]".
-          -- iMod ("HClose" with "[Hkeys]") as "_"; last done.
-             iNext. iExists vo'.
-             rewrite !big_sepM2_insert; try set_solver.
-             iDestruct "Hkeys" as "(Hx & Hy & _)". iFrame.
-          -- iMod ("HClose" with "[Hx Hy]") as "_"; last done.
-             iNext. iExists vo'. iFrame.
-        * iApply ("HΦ'" $! {["x" := (None, false); "y" := (None, false)]}).
-          iSplit. { iPureIntro. set_solver. }
-          iSplitL. {rewrite !big_sepM_insert; try set_solver. rewrite big_sepM_empty. iFrame. }
-          iInv (client_inv_name) as ">[%vo'[Hx Hy]]" "HClose".
-          iModIntro. iExists {["x" := vo'; "y" := vo']}.
-          rewrite !big_sepM_insert; try set_solver.
-          rewrite big_sepM_empty. iFrame.
-          iSplit. { iPureIntro. set_solver. }
-          iSplit. { iPureIntro. set_solver. }
-          iIntros ">[ Hkeys | (Hx & Hy & _)]".
-          -- iMod ("HClose" with "[Hkeys]") as "_"; last done.
-             iNext. iExists vo'.
-             rewrite !big_sepM2_insert; try set_solver.
-             iDestruct "Hkeys" as "(Hx & Hy & _)". iFrame.
-          -- iMod ("HClose" with "[Hx Hy]") as "_"; last done.
-             iNext. iExists vo'. iFrame.
+        rewrite big_sepM_empty. iFrame.
     - iNext. iIntros. by iApply "HΦ".
   Qed.
 
@@ -380,4 +350,4 @@ Proof.
   do 3 (rewrite big_sepS_union; [|set_solver];
   rewrite !big_sepS_singleton;
   iDestruct "Hips" as "[Hips ?]"; iFrame).
-Qed.
+Qed. *)
